rewrite inode in separation logic style

src/Inode.v
@@ -1,3 +1,4 @@
+
 Require Import Arith.
 Require Import Pred.
 Require Import Word.
@@ -16,6 +17,7 @@ Require Import FunctionalExtensionality.
 Require Import NArith.
 Require Import WordAuto.
 Require Import RecArray.
+Require Import GenSep.
 
 Import ListNotations.
 
@@ -35,8 +37,8 @@ Module INODE.
     ("len", Rec.WordF addrlen);
     ("blocks", Rec.ArrayF (Rec.WordF addrlen) blocks_per_inode)]).
 
-  Definition inode := Rec.data inodetype.
-  Definition inode_zero := @Rec.of_word inodetype $0.
+  Definition inode' := Rec.data inodetype.
+  Definition inode0' := @Rec.of_word inodetype $0.
 
   Definition itemsz := Rec.len inodetype.
   Definition items_per_valu : addr := $16.
@@ -45,61 +47,211 @@ Module INODE.
     rewrite valulen_is; auto.
   Qed.
 
-  Definition blocktype : Rec.type := Rec.ArrayF inodetype (wordToNat items_per_valu).
-  Definition block := Rec.data blocktype.
-  Definition block_zero := @Rec.of_word blocktype $0.
-
-  Theorem blocksz : Rec.len blocktype = valulen.
-    rewrite valulen_is; auto.
-  Qed.
-
   Definition xp_to_raxp xp :=
     RecArray.Build_xparams (IXStart xp) (IXLen xp).
 
-  Definition rep xp (ilist : list inode) :=
+  Definition rep' xp (ilist : list inode') :=
     RecArray.array_item inodetype items_per_valu itemsz_ok (xp_to_raxp xp) ilist.
 
-  Definition iget T lxp xp inum rx : prog T :=
+  Definition iget' T lxp xp inum rx : prog T :=
     RecArray.get inodetype items_per_valu itemsz_ok
       lxp (xp_to_raxp xp) inum rx.
 
-  Definition iput T lxp xp inum i rx : prog T :=
+  Definition iput' T lxp xp inum i rx : prog T :=
     RecArray.put inodetype items_per_valu itemsz_ok
       lxp (xp_to_raxp xp) inum i rx.
 
-  Theorem iget_ok : forall lxp xp inum,
-    {< F F' mbase m ilist idata,
+  Theorem iget_ok' : forall lxp xp inum,
+    {< F mbase m ilist,
     PRE    LOG.rep lxp (ActiveTxn mbase m) *
-           [[ (F * rep xp ilist)%pred m ]] *
-           [[ (F' * inum |-> idata)%pred (list2mem ilist) ]]
-    POST:r LOG.rep lxp (ActiveTxn mbase m) * [[ r = idata ]]
+           [[ (F * rep' xp ilist)%pred m ]] *
+           [[ (inum < IXLen xp ^* items_per_valu)%word ]]
+    POST:r LOG.rep lxp (ActiveTxn mbase m) *
+           [[ r = sel ilist inum inode0' ]]
     CRASH  LOG.log_intact lxp mbase
-    >} iget lxp xp inum.
+    >} iget' lxp xp inum.
   Proof.
-    unfold iget, rep.
+    unfold iget', rep'.
     intros. eapply pimpl_ok2. eapply RecArray.get_ok; word_neq.
     step.
   Qed.
 
-  Theorem iput_ok : forall lxp xp inum i,
-    {< F F' mbase m ilist oldidata,
+  Theorem iput_ok' : forall lxp xp inum i,
+    {< F mbase m ilist,
     PRE    LOG.rep lxp (ActiveTxn mbase m) *
-           [[ (F * rep xp ilist)%pred m ]] *
-           [[ (F' * inum |-> oldidata)%pred (list2mem ilist) ]] *
+           [[ (F * rep' xp ilist)%pred m ]] *
+           [[ (inum < IXLen xp ^* items_per_valu)%word ]] *
            [[ Rec.well_formed i ]]
     POST:r ([[ r = false ]] * LOG.rep lxp (ActiveTxn mbase m)) \/
-           ([[ r = true ]] * exists m' ilist', LOG.rep lxp (ActiveTxn mbase m') *
-            [[ (F * rep xp ilist')%pred m' ]] *
-            [[ (F' * inum |-> i)%pred (list2mem ilist) ]])
+           ([[ r = true ]] * exists m', LOG.rep lxp (ActiveTxn mbase m') *
+            [[ (F * rep' xp (upd ilist inum i))%pred m' ]])
     CRASH  LOG.log_intact lxp mbase
-    >} iput lxp xp inum i.
+    >} iput' lxp xp inum i.
   Proof.
-    unfold iput, rep.
+    unfold iput', rep'.
     intros. eapply pimpl_ok2. eapply RecArray.put_ok; word_neq.
     step.
   Qed.
 
-  Hint Extern 1 ({{_}} progseq (iget _ _ _) _) => apply iget_ok : prog.
-  Hint Extern 1 ({{_}} progseq (iput _ _ _ _) _) => apply iput_ok : prog.
+  Hint Extern 1 ({{_}} progseq (iget' _ _ _) _) => apply iget_ok' : prog.
+  Hint Extern 1 ({{_}} progseq (iput' _ _ _ _) _) => apply iput_ok' : prog.
+
+
+  (* separation logic based theorems *)
+
+  Record inode := {
+    IBlocks : list addr
+    (* add indirect link later *)
+  }.
+
+  Definition inode0 := Build_inode nil.
+
+  Definition igetlen T lxp xp inum rx : prog T :=
+    i <- iget' lxp xp inum;
+    rx (i :-> "len").
+
+  Definition iget T lxp xp inum off rx : prog T :=
+    i <- iget' lxp xp inum ;
+    rx (sel (i :-> "blocks") off $0).
+
+  Definition iput T lxp xp inum off a rx : prog T :=
+    i <- iget' lxp xp inum ;
+    let i' := i :=> "blocks" := (upd (i :-> "blocks") off a) in
+    iput' lxp xp inum i' rx.
+
+  Definition igrow T lxp xp inum a rx : prog T :=
+    i <- iget' lxp xp inum ;
+    let i' := i :=> "blocks" := (upd (i :-> "blocks") (i :-> "len") a) in
+    let i'' := i' :=> "len" := (i' :-> "len" ^+ $1) in
+    iput' lxp xp inum i'' rx.
+
+  Definition ishrink T lxp xp inum rx : prog T :=
+    i <- iget' lxp xp inum ;
+    let i' := i :=> "len" := (i :-> "len" ^- $1) in
+    iput' lxp xp inum i' rx.
+
+  Definition blocks_match i (i' : inode') :=
+    forall off, off < length (IBlocks i)
+    -> selN (IBlocks i) off $0 = selN (i' :-> "blocks") off $0.
+
+  Definition inode_match i (i' : inode') :=
+    (exists (b : addr), length (IBlocks i) <= wordToNat b) /\
+    length (IBlocks i) = wordToNat (i' :-> "len") /\
+    blocks_match i i'.
+
+  Definition rep xp (ilist : list inode) :=
+    (exists ilist', rep' xp ilist' *
+     [[ length ilist = length ilist' ]] * 
+     [[ forall i, inode_match (selN ilist i inode0) (selN ilist' i inode0') ]])%pred.
+
+  Definition inum_valid inum xp (ilist : list inode) :=
+      (inum < IXLen xp ^* items_per_valu)%word /\
+      wordToNat inum < length ilist.
+
+  Definition off_valid (off : addr) ino :=
+    wordToNat off < length (IBlocks ino).
+
+  Hint Unfold inum_valid.
+  Hint Unfold off_valid.
+
+
+  Ltac destruct_hyp H := match type of H with
+    | _ /\ _ => let X := fresh in
+              destruct H as [H X]; destruct_hyp H; destruct_hyp X
+    | ex _ => destruct H
+    | _ => idtac
+  end.
+
+  Ltac specialize_inode_match inum := match goal with
+    | [ H: forall _, inode_match _ _ |- _ ] =>
+      let X := fresh in 
+          pose proof (H (wordToNat inum)) as X;
+          unfold inode_match in X;
+          destruct_hyp X; clear H
+  end.
+
+  Ltac specialize_inode_match_off inum off := match goal with
+    | [ H: forall _, inode_match _ _ |- _ ] =>
+         specialize_inode_match inum; 
+         match goal with
+           | [ H: blocks_match _ _ |- _ ] =>
+             let X := fresh in
+                unfold blocks_match in H;
+                pose proof (H (wordToNat off)) as X; clear H
+          end
+  end.
+
+  Ltac inode_simpl' := match goal with
+    | [ H: (_ * ?inum |-> ?i)%pred (list2mem ?il) |- context [?i] ] =>
+      match type of i with
+      | inode => replace i with (sel il inum inode0) by (erewrite list2mem_sel; eauto)
+      | addr => replace i with (sel il inum $0) by (erewrite list2mem_sel; eauto)
+      end
+    | [ H: (_ * ?inum |-> ?i)%pred (list2mem ?il), H2: context [?i] |- _ ] =>
+      match type of i with
+      | inode => replace i with (sel il inum inode0) in H2 by (erewrite list2mem_sel; eauto)
+      | addr => replace i with (sel il inum $0) in H2 by (erewrite list2mem_sel; eauto)
+      end
+  end.
+
+  Ltac inode_simpl := repeat inode_simpl'; subst.
+
+  Theorem igetlen_ok : forall lxp xp inum,
+    {< F A mbase m ilist ino,
+    PRE    LOG.rep lxp (ActiveTxn mbase m) *
+           [[ inum_valid inum xp ilist ]] *
+           [[ (F * rep xp ilist)%pred m ]] *
+           [[ (A * inum |-> ino)%pred (list2mem ilist) ]]
+    POST:r LOG.rep lxp (ActiveTxn mbase m) * [[ r = $ (length (IBlocks ino)) ]]
+    CRASH  LOG.log_intact lxp mbase
+    >} igetlen lxp xp inum.
+  Proof.
+    unfold igetlen, rep, inum_valid.
+    hoare.
+
+    specialize_inode_match inum.
+    inode_simpl.
+    apply wordToNat_inj; erewrite wordToNat_natToWord_bound; eauto.
+  Qed.
+
+  Theorem iget_ok : forall lxp xp inum off,
+    {< F A B mbase m ilist ino a,
+    PRE    LOG.rep lxp (ActiveTxn mbase m) *
+           [[ inum_valid inum xp ilist /\ off_valid off ino ]] *
+           [[ (F * rep xp ilist)%pred m ]] *
+           [[ (A * inum |-> ino)%pred (list2mem ilist) ]] *
+           [[ (B * off |-> a)%pred (list2mem (IBlocks ino)) ]]
+    POST:r LOG.rep lxp (ActiveTxn mbase m) * [[ r = a ]]
+    CRASH  LOG.log_intact lxp mbase
+    >} iget lxp xp inum off.
+  Proof.
+    unfold iget, rep, inum_valid, off_valid.
+    hoare.
+    specialize_inode_match_off inum off.
+    inode_simpl.
+    intuition.
+  Qed.
+
+  Theorem iput_ok : forall lxp xp inum off a,
+    {< F A B mbase m ilist ino,
+    PRE    LOG.rep lxp (ActiveTxn mbase m) *
+           [[ inum_valid inum xp ilist /\ off_valid off ino ]] *
+           [[ (F * rep xp ilist)%pred m ]] *
+           [[ (A * inum |-> ino)%pred (list2mem ilist) ]] *
+           [[ (B * off |->?)%pred (list2mem (IBlocks ino)) ]]
+    POST:r ([[ r = false ]] * LOG.rep lxp (ActiveTxn mbase m)) \/
+           ([[ r = true ]] * exists m' ilist' ino',
+            LOG.rep lxp (ActiveTxn mbase m') *
+            [[ (F * rep xp ilist')%pred m' ]] *
+            [[ (A * inum |-> ino')%pred (list2mem ilist') ]] *
+            [[ (B * off |-> a)%pred (list2mem (IBlocks ino')) ]])
+    CRASH  LOG.log_intact lxp mbase
+    >} iput lxp xp inum off a.
+  Proof.
+    unfold iput, rep, inum_valid, off_valid.
+    hoare.
+    admit.
+  Qed.
+
 
 End INODE.
